src/Writer.fst
@@ -1,0 +1,23 @@
+module Writer
+
+open Reader
+open Ring
+open FStar.HyperStack
+open FStar.HyperStack.ST
+open FStar.UInt32
+module B = LowStar.Buffer
+open LowStar.BufferOps
+
+
+abstract let writer (r: ringstruct8) (v:message) : ST ringstruct8
+  (requires fun h -> 
+     live_rb h r
+     /\ well_formed_rb r
+  )
+  (ensures fun h0 res h1 -> 
+  live_rb h1 res
+  /\ well_formed_rb res) 
+  =
+  let (r', s) = (Ring.push r v) in
+  r'
+  
